Ported most of LambdaOmega to universes; 4 problems left to solve

examples/metatheory/LambdaOmega.fst
@@ -81,7 +81,7 @@ val esub_lam_renaming: s:esub -> Lemma
 let esub_lam_renaming s = ()
 
 (* Substitution extensional; trivial with the extensionality axiom *)
-val esubst_extensional: s1:esub -> s2:esub{FEq s1 s2} -> e:exp ->
+val esubst_extensional: s1:esub -> s2:esub{feq s1 s2} -> e:exp ->
                         Lemma (requires True) (ensures (esubst s1 e = esubst s2 e))
                        (*[SMTPat (esubst s1 e);  SMTPat (esubst s2 e)]*)
 let esubst_extensional s1 s2 e = ()
@@ -151,7 +151,7 @@ let tsub_lam s y =
            else tsubst tsub_inc (s (y-1))
 
 (* Type substitution extensional; trivial with the extensionality axiom *)
-val tsubst_extensional: s1:tsub -> s2:tsub{FEq s1 s2} -> t:typ ->
+val tsubst_extensional: s1:tsub -> s2:tsub{feq s1 s2} -> t:typ ->
                         Lemma (requires True) (ensures (tsubst s1 t = tsubst s2 t))
 (*                       [SMTPat (tsubst t s1);  SMTPat (tsubst t s2)]*)
 let tsubst_extensional s1 s2 t = ()
@@ -177,7 +177,7 @@ val tsub_lam_renaming: s:tsub -> Lemma
 let tsub_lam_renaming s = ()
 
 val tsubst_comp : s1:tsub -> s2:tsub -> t:typ -> Lemma
-      (tsubst s1 (tsubst s2 t) = tsubst (tsub_comp s1 s2) t)
+      (ensures (tsubst s1 (tsubst s2 t) = tsubst (tsub_comp s1 s2) t))
       (decreases %[is_tvar t;
                    is_trenaming s1;
                    is_trenaming s2;
@@ -214,7 +214,7 @@ let rec tsubst_comp s1 s2 t =
 
     let h2 =
       forall_intro tsub_lam_comp;
-      cut (FEq (tsub_comp (tsub_lam s1) (tsub_lam s2))
+      cut (feq (tsub_comp (tsub_lam s1) (tsub_lam s2))
              (tsub_lam (tsub_comp s1 s2))) in
 
     let ext = tsubst_extensional
@@ -292,12 +292,12 @@ type step : exp -> exp -> Type =
   | SApp1 : #e1:exp ->
              e2:exp ->
             #e1':exp ->
-            =hst:(step e1 e1') ->
+            $hst:(step e1 e1') ->
              step (EApp e1 e2) (EApp e1' e2)
   | SApp2 :  e1:exp ->
             #e2:exp ->
             #e2':exp ->
-            =hst:(step e2 e2') ->
+            $hst:(step e2 e2') ->
              step (EApp e1 e2) (EApp e1 e2')
 
 (* Typing environments *)
@@ -325,10 +325,10 @@ let empty = MkEnv empty_a empty_x
 
 val extend_tvar: g:env -> n:nat -> k:knd -> Tot env
 let extend_tvar g n k =
-  let a_env = fun a -> if a < n then lookup_tvar g a
-                       else if a = n then Some k
-                       else lookup_tvar g (a - 1) in
-  let x_env = fun x -> match lookup_evar g x with
+  let a_env = fun (a:nat) -> if a < n then lookup_tvar g a
+                             else if a = n then Some k
+                             else lookup_tvar g (a - 1) in
+  let x_env = fun (x:nat) -> match lookup_evar g x with
     | None -> None
     | Some t -> Some (tshift_up_above n t)
   in
@@ -336,10 +336,10 @@ let extend_tvar g n k =
 
 val extend_evar: g:env -> n:nat -> t:typ -> Tot env
 let extend_evar g n t =
-  let a_env = fun a -> lookup_tvar g a in
-  let x_env = fun x -> if x < n then lookup_evar g x
-                       else if x = n then Some t
-                       else lookup_evar g (x - 1) in
+  let a_env = fun (a:nat) -> lookup_tvar g a in
+  let x_env = fun (x:nat) -> if x < n then lookup_evar g x
+                             else if x = n then Some t
+                             else lookup_evar g (x - 1) in
   MkEnv a_env x_env
 
 (* Kinding, type equivalence, and typing rules;
@@ -353,21 +353,21 @@ type kinding : env -> typ -> knd -> Type =
              k:knd ->
             #t:typ ->
             #k':knd ->
-            =hk:kinding (extend_tvar g 0 k) t k' ->
+            $hk:kinding (extend_tvar g 0 k) t k' ->
                 kinding g (TLam k t) (KArr k k')
   | KiApp : #g:env ->
             #t1:typ ->
             #t2:typ ->
             #k11:knd ->
             #k12:knd ->
-            =hk1:kinding g t1 (KArr k11 k12) ->
-            =hk2:kinding g t2 k11 ->
+            $hk1:kinding g t1 (KArr k11 k12) ->
+            $hk2:kinding g t2 k11 ->
                  kinding g (TApp t1 t2) k12
   | KiArr : #g:env ->
             #t1:typ ->
             #t2:typ ->
-            =hk1:kinding g t1 KTyp ->
-            =hk2:kinding g t2 KTyp ->
+            $hk1:kinding g t1 KTyp ->
+            $hk2:kinding g t2 KTyp ->
                  kinding g (TArr t1 t2) KTyp
 
 type tequiv : typ -> typ -> Type =
@@ -375,25 +375,25 @@ type tequiv : typ -> typ -> Type =
              tequiv t t
   | EqSymm : #t1:typ ->
              #t2:typ ->
-             =he:tequiv t1 t2 ->
+             $he:tequiv t1 t2 ->
              tequiv t2 t1
   | EqTran : #t1:typ ->
              #t2:typ ->
              #t3:typ ->
-             =he12:tequiv t1 t2 ->
-             =he23:tequiv t2 t3 ->
+             $he12:tequiv t1 t2 ->
+             $he23:tequiv t2 t3 ->
                    tequiv t1 t3
   | EqLam : #t :typ ->
             #t':typ ->
              k :knd ->
-            =he:tequiv t t' ->
+            $he:tequiv t t' ->
                 tequiv (TLam k t) (TLam k t')
   | EqApp : #t1 :typ ->
             #t1':typ ->
             #t2 :typ ->
             #t2':typ ->
-            =he1:tequiv t1 t1' ->
-            =he2:tequiv t2 t2' ->
+            $he1:tequiv t1 t1' ->
+            $he2:tequiv t2 t2' ->
                  tequiv (TApp t1 t2) (TApp t1' t2')
   | EqBeta :k:knd ->
             t1:typ ->
@@ -403,37 +403,37 @@ type tequiv : typ -> typ -> Type =
             #t1':typ ->
             #t2 :typ ->
             #t2':typ ->
-            =he1:tequiv t1 t1' ->
-            =he2:tequiv t2 t2' ->
+            $he1:tequiv t1 t1' ->
+            $he2:tequiv t2 t2' ->
                  tequiv (TArr t1 t2) (TArr t1' t2')
 
 type typing : env -> exp -> typ -> Type =
   | TyVar : #g:env ->
              x:var{is_Some (lookup_evar g x)} ->
-            =hk:kinding g (Some.v (lookup_evar g x)) KTyp ->
+            $hk:kinding g (Some.v (lookup_evar g x)) KTyp ->
                 typing g (EVar x) (Some.v (lookup_evar g x))
   | TyLam : #g:env ->
              t:typ ->
             #e1:exp ->
             #t':typ ->
-            =hk:kinding g t KTyp ->
-            =ht:typing (extend_evar g 0 t) e1 t' ->
+            $hk:kinding g t KTyp ->
+            $ht:typing (extend_evar g 0 t) e1 t' ->
                 typing g (ELam t e1) (TArr t t')
   | TyApp : #g:env ->
             #e1:exp ->
             #e2:exp ->
             #t1:typ ->
             #t2:typ ->
-            =ht1:typing g e1 (TArr t1 t2) ->
-            =ht2:typing g e2 t1 ->
+            $ht1:typing g e1 (TArr t1 t2) ->
+            $ht2:typing g e2 t1 ->
                  typing g (EApp e1 e2) t2
   | TyEqu : #g:env ->
             #e:exp ->
             #t1:typ ->
             #t2:typ ->
-            =ht:typing g e t1 ->
-            =he:tequiv t1 t2 ->
-            =hk:kinding g t2 KTyp ->
+            $ht:typing g e t1 ->
+            $he:tequiv t1 t2 ->
+            $hk:kinding g t2 KTyp ->
                 typing g e t2
 
 (* Progress proof *)
@@ -443,16 +443,19 @@ let is_value = is_ELam
 
 opaque val progress : #e:exp -> #t:typ -> h:typing empty e t ->
                Pure (cexists (fun e' -> step e e'))
-                    (requires (not (is_value e)))
+                    (requires (b2t (not (is_value e))))
                     (ensures (fun _ -> True)) (decreases h)
-let rec progress _ _ h =
+let rec progress #e #t h =
   match h with
     | TyApp #g #e1 #e2 #t11 #t12 h1 h2 ->
       (match e1 with
        | ELam t e1' -> ExIntro (esubst_beta e2 e1') (SBeta t e1' e2)
        | _ -> (match progress h1 with
-                | ExIntro e1' h1' -> ExIntro (EApp e1' e2) (SApp1 e2 h1')))
-    | TyEqu h1 _ _ -> progress h1
+               | ExIntro e1' h1' -> ExIntro (EApp e1' e2) (SApp1 e2 h1')))
+    (* | TyEqu h1 _ _ -> progress h1 -- used to work *)
+    (* | TyEqu #g #e #t1 #t2 h1 _ _ -> progress #e #t1 h1
+       -- explicit annotation does't help*)
+       | TyEqu h1 _ _ -> magic() (* XXX; filed at #579 *)
 
 val tappears_free_in : x:var -> t:typ -> Tot bool (decreases t)
 let rec tappears_free_in x t =
@@ -462,14 +465,14 @@ let rec tappears_free_in x t =
   | TApp t1 t2 -> tappears_free_in x t1 || tappears_free_in x t2
   | TLam _ t1 -> tappears_free_in (x+1) t1
 
-opaque logic type EnvEqualT (t:typ) (g1:env) (g2:env) =
+opaque logic type envEqualT (t:typ) (g1:env) (g2:env) =
                  (forall (x:var). tappears_free_in x t ==>
                     lookup_tvar g1 x = lookup_tvar g2 x)
 
 opaque val tcontext_invariance : #t:typ -> #g:env -> #k:knd ->
-                          h:(kinding g t k) -> g':env{EnvEqualT t g g'} ->
+                          h:(kinding g t k) -> g':env{envEqualT t g g'} ->
                           Tot (kinding g' t k) (decreases h)
-let rec tcontext_invariance _ _ _ h g' =
+let rec tcontext_invariance #t #g #k h g' =
   match h with
   | KiVar a -> KiVar a
   | KiLam k1 h1 -> KiLam k1 (tcontext_invariance h1 (extend_tvar g' 0 k1))
@@ -479,9 +482,9 @@ let rec tcontext_invariance _ _ _ h g' =
        because (MkEnv.x g) and (MkEnv.x g') are completely unrelated;
        this is just because we pass this useless argument to kinding. *)
 opaque val kinding_extensional: #g:env -> #t:typ -> #k:knd -> h:(kinding g t k) ->
-                g':env{FEq (MkEnv.a g) (MkEnv.a g')} ->
+                g':env{feq (MkEnv.a g) (MkEnv.a g')} ->
                 Tot (kinding g' t k) (decreases h)
-let rec kinding_extensional _ _ _ h g' =
+let rec kinding_extensional #g #t #k h g' =
   match h with
     | KiVar a -> KiVar a
     | KiLam k1 h1 -> KiLam k1 (kinding_extensional h1 (extend_tvar g' 0 k1))
@@ -492,7 +495,7 @@ let rec kinding_extensional _ _ _ h g' =
 opaque val kinding_weakening_ebnd : #g:env -> #t:typ -> #k:knd ->
       h:(kinding g t k) -> x:var -> t':typ ->
       Tot (kinding (extend_evar g x t') t k)
-let kinding_weakening_ebnd g t k h x t' =
+let kinding_weakening_ebnd #g #t #k h x t' =
   kinding_extensional h (extend_evar g x t')
 
 val tshift_up_above_lam: n:nat -> k:knd -> t:typ -> Lemma
@@ -508,7 +511,7 @@ let tshift_up_above_lam n k t =
 opaque val kinding_weakening_tbnd : #g:env -> #t:typ -> #k:knd ->
       h:(kinding g t k) -> x:var -> k':knd ->
       Tot (kinding (extend_tvar g x k') (tshift_up_above x t) k) (decreases h)
-let rec kinding_weakening_tbnd g t k h x k' =
+let rec kinding_weakening_tbnd #g #t #k h x k' =
   match h with
     | KiVar a -> if a < x then KiVar a
                           else KiVar (a + 1)
@@ -527,18 +530,18 @@ opaque val kinding_strengthening_ebnd :
       g:env -> x:var -> t_x:typ -> #t:typ -> #k:knd ->
       h:(kinding (extend_evar g x t_x) t k) ->
       Tot (kinding g t k) (decreases h)
-let kinding_strengthening_ebnd g x t_x t k h = kinding_extensional h g
+let kinding_strengthening_ebnd g x t_x #t #k h = kinding_extensional h g
 
 opaque val kinding_inversion_arrow: #g:env -> #t1:typ -> #t2:typ ->
                              h:(kinding g (TArr t1 t2) KTyp) ->
                              Tot (cand (kinding g t1 KTyp) (kinding g t2 KTyp))
-let rec kinding_inversion_arrow g t1 t2 h = match h with
+let rec kinding_inversion_arrow #g #t1 #t2 h = match h with
   | KiArr h1 h2 -> Conj h1 h2
 
 opaque val typing_to_kinding : #g:env -> #e:exp -> #t:typ ->
                                     h:(typing g e t) ->
                                     Tot (kinding g t KTyp) (decreases h)
-let rec typing_to_kinding g e t h = match h with
+let rec typing_to_kinding #g #e #t h = match h with
   | TyVar x h -> h
   | TyLam t' hk h1 -> KiArr hk (kinding_strengthening_ebnd g 0 t'
                                   (typing_to_kinding h1))
@@ -587,7 +590,7 @@ let rec tshift_up_above_tsubst_beta x t1 t2 =
 opaque val tequiv_tshift : #t1:typ -> #t2:typ -> h:(tequiv t1 t2) -> x:nat ->
                Tot (tequiv (tshift_up_above x t1) (tshift_up_above x t2))
                (decreases h)
-let rec tequiv_tshift t1 t2 h x =
+let rec tequiv_tshift #t1 #t2 h x =
   match h with
   | EqRefl t -> EqRefl (tshift_up_above x t)
   | EqSymm h1 -> EqSymm (tequiv_tshift h1 x)
@@ -615,7 +618,7 @@ type subst_typing (s:esub) (g1:env) (g2:env) =
   f:(x:var{is_Some (lookup_evar g1 x)} ->
      kinding g1 (Some.v (lookup_evar g1 x)) KTyp ->
      Tot(typing g2 (s x) (Some.v (lookup_evar g1 x)))
-    ){FEq (MkEnv.a g1) (MkEnv.a g2)}
+    ){feq (MkEnv.a g1) (MkEnv.a g2)}
 
 opaque val substitution :
       #g1:env -> #e:exp -> #t:typ -> s:esub -> #g2:env ->
@@ -623,24 +626,25 @@ opaque val substitution :
       hs:subst_typing s g1 g2 ->
       Tot (typing g2 (esubst s e) t)
      (decreases %[is_var e; is_renaming s; h1])
-let rec substitution g1 e t s g2 h1 hs =
+let rec substitution #g1 #e #t s #g2 h1 hs =
   match h1 with
   | TyVar x kind_normal -> hs x kind_normal
   | TyApp hfun harg -> TyApp (substitution s hfun hs) (substitution s harg hs)
   | TyLam #gtemp tlam #ebody #tfun hkind hbody ->
-     let hs'' : subst_typing (esub_inc) (g2) (extend_evar g2 0 tlam) =
-       fun x hkind ->
-         TyVar (x+1) (kinding_extensional hkind (extend_evar g2 0 tlam)) in
-     let hs' : subst_typing (esub_lam s) (extend_evar g1 0 tlam)
-                                         (extend_evar g2 0 tlam) =
-       fun y hkindg1 ->
-         if y = 0
-         then TyVar y (kinding_extensional hkindg1 (extend_evar g2 0 tlam))
-         else let hgamma2 = hs (y - 1) (kinding_extensional hkindg1 g1) in
-              substitution esub_inc hgamma2 hs''
-     in (esub_lam_hoist tlam ebody s;
-         TyLam tlam (kinding_extensional hkind g2)
-               (substitution (esub_lam s) hbody hs'))
+     magic() (* XXX *)
+     (* let hs'' : subst_typing (esub_inc) (g2) (extend_evar g2 0 tlam) = *)
+     (*   fun (x:var) hkind -> *)
+     (*     TyVar (x+1) (kinding_extensional hkind (extend_evar g2 0 tlam)) in *)
+     (* let hs' : subst_typing (esub_lam s) (extend_evar g1 0 tlam) *)
+     (*                                     (extend_evar g2 0 tlam) = *)
+     (*   fun (y:var) hkindg1 -> *)
+     (*     if y = 0 *)
+     (*     then TyVar y (kinding_extensional hkindg1 (extend_evar g2 0 tlam)) *)
+     (*     else let hgamma2 = hs (y - 1) (kinding_extensional hkindg1 g1) in *)
+     (*          substitution esub_inc hgamma2 hs'' *)
+     (* in (esub_lam_hoist tlam ebody s; *)
+     (*     TyLam tlam (kinding_extensional hkind g2) *)
+     (*           (substitution (esub_lam s) hbody hs')) *)
   | TyEqu het1 hequiv hkind ->
      TyEqu (substitution s het1 hs) hequiv (kinding_extensional hkind g2)
 
@@ -649,7 +653,7 @@ opaque val typing_substitution: #e:exp -> #v:exp -> #t_x:typ ->
       h1:(typing g v t_x) ->
       h2:(typing (extend_evar g 0 t_x) e t) ->
       Tot (typing g (esubst_beta v e) t) (decreases %[e;h2])
-let rec typing_substitution e v t_x t g h1 h2 =
+let rec typing_substitution #e #v #t_x #t #g h1 h2 =
   let hs : subst_typing (esub_beta v) (extend_evar g 0 t_x) g =
     fun y hkind -> if y = 0 then h1
                    else TyVar (y-1) (kinding_extensional hkind g) in
@@ -701,29 +705,29 @@ type tred: typ -> typ -> Type =
            tred t t
 
   | TrArr:  #t1:typ -> #t2:typ -> #t1':typ -> #t2':typ ->
-            =hr1:tred t1 t1' ->
-            =hr2:tred t2 t2' ->
+            $hr1:tred t1 t1' ->
+            $hr2:tred t2 t2' ->
                  tred (TArr t1 t2) (TArr t1' t2')
 
   | TrLam:  #t1:typ -> #t2:typ -> k:knd ->
-            =hr:tred t1 t2 ->
+            $hr:tred t1 t2 ->
                 tred (TLam k t1) (TLam k t2)
 
   | TrApp:  #t1:typ -> #t2:typ -> #t1':typ -> #t2':typ ->
-            =hr1:tred t1 t1' ->
-            =hr2:tred t2 t2' ->
+            $hr1:tred t1 t1' ->
+            $hr2:tred t2 t2' ->
                  tred (TApp t1 t2) (TApp t1' t2')
 
   | TrBeta: #t1:typ -> #t2:typ -> #t1':typ -> #t2':typ -> k:knd ->
-            =hr1:tred t1 t1' ->
-            =hr2:tred t2 t2' ->
+            $hr1:tred t1 t1' ->
+            $hr2:tred t2 t2' ->
                  tred (TApp (TLam k t1) t2) (tsubst_beta t2' t1')
 
 (* t => t' implies tshift_up_above x t => tshift_up_above x t' *)
 opaque val tred_shiftup_above: #t:typ -> #t':typ -> x:nat -> h:(tred t t') ->
                         Tot (tred (tshift_up_above x t) (tshift_up_above x t'))
                         (decreases h)
-let rec tred_shiftup_above t t' x h =
+let rec tred_shiftup_above #t #t' x h =
   match h with
     | TrRefl t''  -> TrRefl (tshift_up_above x t'')
     | TrArr h1 h2 -> TrArr (tred_shiftup_above x h1) (tred_shiftup_above x h2)
@@ -742,7 +746,7 @@ opaque val subst_of_tred: #s:typ -> #s':typ -> x:nat -> t:typ ->
                    h:(tred s s') ->
                    Tot (tred (tsubst_beta_gen x s t) (tsubst_beta_gen x s' t))
                    (decreases t)
-let rec subst_of_tred s s' x t h =
+let rec subst_of_tred #s #s' x t h =
   match t with
     | TVar y -> if y < x then TrRefl t
                 else if y = x then h
@@ -792,7 +796,7 @@ opaque val subst_of_tred_tred: #s:typ -> #s':typ -> #t:typ -> #t':typ -> x:nat -
                        hs:(tred s s') -> ht:(tred t t') ->
                        Tot (tred (tsubst_beta_gen x s t) (tsubst_beta_gen x s' t'))
                        (decreases ht)
-let rec subst_of_tred_tred s s' t t' x hs ht =
+let rec subst_of_tred_tred #s #s' #t #t' x hs ht =
   match ht with
     | TrRefl t1 -> subst_of_tred x t1 hs
     | TrArr ht1 ht2 ->
@@ -811,14 +815,14 @@ let rec subst_of_tred_tred s s' t t' x hs ht =
       TrBeta k ht1' ht2'
 
 type ltup =
-  | MkLTup: #s:typ -> #t:typ -> #u:typ -> =h1:(tred s t) -> =h2:(tred s u) -> ltup
+  | MkLTup: #s:typ -> #t:typ -> #u:typ -> $h1:(tred s t) -> $h2:(tred s u) -> ltup
 
 (* single step diamond property of parallel reduction *)
 opaque val tred_diamond: #s:typ -> #t:typ -> #u:typ ->
                   h1:(tred s t) -> h2:(tred s u) ->
                   Tot (cexists (fun v -> cand (tred t v) (tred u v)))
                   (decreases %[h1;h2])
-let rec tred_diamond s t u h1 h2 =
+let rec tred_diamond #s #t #u h1 h2 =
   match (MkLTup h1 h2) with
     | MkLTup (TrRefl t1) _ -> ExIntro u (Conj h2 (TrRefl u))
     | MkLTup _ (TrRefl t1) -> ExIntro t (Conj (TrRefl t) h1)
@@ -853,10 +857,11 @@ let rec tred_diamond s t u h1 h2 =
         match h21 with
           | TrLam _ h' -> h'
           | TrRefl _ -> TrRefl (TLam.t s1') in
-      let ExIntro v1 (Conj p1a p1b) = tred_diamond h11 h21 in
-      let ExIntro v2 (Conj p2a p2b) = tred_diamond h12 h22 in
-      let v = tsubst_beta v2 v1 in
-      ExIntro v (Conj (subst_of_tred_tred 0 p2a p1a) (TrBeta k p1b p2b))
+      magic() (* XXX *)
+      (* let ExIntro v1 (Conj p1a p1b) = tred_diamond h11 h21 in *)
+      (* let ExIntro v2 (Conj p2a p2b) = tred_diamond h12 h22 in *)
+      (* let v = tsubst_beta v2 v1 in *)
+      (* ExIntro v (Conj (subst_of_tred_tred 0 p2a p1a) (TrBeta k p1b p2b)) *)
 
     | MkLTup (TrApp #s1' #s2' #lu1' #u2' h21 h22)
              (TrBeta #s1 #s2 #t1' #t2' k h11 h12) ->
@@ -870,22 +875,23 @@ let rec tred_diamond s t u h1 h2 =
         match p2 with
           | TrLam _ h' -> h'
           | TrRefl _ -> TrRefl t1' in
-      ExIntro (tsubst_beta v2 (TLam.t v1))
-              (Conj (TrBeta k h_body p3) (subst_of_tred_tred 0 p4 h_body2))
+      magic() (* XXX *)
+      (* ExIntro (tsubst_beta v2 (TLam.t v1)) *)
+      (*         (Conj (TrBeta k h_body p3) (subst_of_tred_tred 0 p4 h_body2)) *)
 
 type tred_star: typ -> typ -> Type =
   | TsRefl : t:typ ->
              tred_star t t
 
   | TsStep : #t1:typ -> #t2:typ -> #t3:typ ->
-             =hr12:tred      t1 t2 ->
-             =hr23:tred_star t2 t3 ->
+             $hr12:tred      t1 t2 ->
+             $hr23:tred_star t2 t3 ->
                    tred_star t1 t3
 
 opaque val tred_star_one_loop: #s:typ -> #t:typ -> #u:typ ->
       h:(tred s t) -> hs:(tred_star s u) ->
       Tot (cexists (fun v -> cand (tred_star t v) (tred u v))) (decreases hs)
-let rec tred_star_one_loop s t u h hs = match hs with
+let rec tred_star_one_loop #s #t #u h hs = match hs with
   | TsRefl _ ->
     ExIntro t (Conj (TsRefl t) h)
   | TsStep #s #u1 #u h1 hs' ->
@@ -898,7 +904,7 @@ opaque val confluence : #s:typ -> #t:typ -> #u:typ ->
       h1:(tred_star s t) -> h2:(tred_star s u) ->
       Tot (cexists (fun v -> cand (tred_star t v) (tred_star u v)))
       (decreases h1)
-let rec confluence s t u h1 h2 =
+let rec confluence #s #t #u h1 h2 =
   match h1 with
   | TsRefl _ ->
     ExIntro u (Conj h2 (TsRefl u))
@@ -910,7 +916,7 @@ let rec confluence s t u h1 h2 =
 opaque val ts_tran: #s:typ -> #t:typ -> #u:typ ->
              h1:tred_star s t -> h2:tred_star t u -> Tot (tred_star s u)
              (decreases h1)
-let rec ts_tran s t u h1 h2 =
+let rec ts_tran #s #t #u h1 h2 =
   match h1 with
     | TsRefl _ -> h2
     | TsStep #s #s1 #t h11 h12 ->
@@ -918,21 +924,21 @@ let rec ts_tran s t u h1 h2 =
 
 type tred_star_sym : typ -> typ -> Type =
   | TssBase: #t1:typ -> #t2:typ ->
-             =hr:tred t1 t2 ->
+             $hr:tred t1 t2 ->
                  tred_star_sym t1 t2
   | TssSym: #t1:typ -> #t2:typ ->
-            =hr:tred_star_sym t2 t1 ->
+            $hr:tred_star_sym t2 t1 ->
                 tred_star_sym t1 t2
   | TssTran: #t1:typ -> #t2:typ -> #t3:typ ->
-             =hr12:tred_star_sym t1 t2 ->
-             =hr23:tred_star_sym t2 t3 ->
+             $hr12:tred_star_sym t1 t2 ->
+             $hr23:tred_star_sym t2 t3 ->
                    tred_star_sym t1 t3
 
 (* Proposition 30.3.10 in TAPL (has a graphical proof only for this, pg. 561) *)
 opaque val tred_star_sym_confluent : #s:typ -> #t:typ ->
       h:tred_star_sym s t ->
       Tot (cexists (fun u -> cand (tred_star s u) (tred_star t u))) (decreases h)
-let rec tred_star_sym_confluent s t h =
+let rec tred_star_sym_confluent #s #t h =
   match h with
     | TssBase h1 -> ExIntro t (Conj (TsStep h1 (TsRefl t)) (TsRefl t))
     | TssSym h1 ->
@@ -947,7 +953,7 @@ let rec tred_star_sym_confluent s t h =
 opaque val trlam_tss : #t1:typ -> #t2:typ -> k:knd ->
       h:(tred_star_sym t1 t2) ->
       Tot (tred_star_sym (TLam k t1) (TLam k t2)) (decreases h)
-let rec trlam_tss t1 t2 k h =
+let rec trlam_tss #t1 #t2 k h =
   match h with
     | TssBase h1 -> TssBase (TrLam k h1)
     | TssSym h1 -> TssSym (trlam_tss k h1)
@@ -956,7 +962,7 @@ let rec trlam_tss t1 t2 k h =
 opaque val trapp_tss_1 : #t1:typ -> t2:typ -> #t1':typ ->
       h:(tred_star_sym t1 t1') ->
       Tot (tred_star_sym (TApp t1 t2) (TApp t1' t2)) (decreases h)
-let rec trapp_tss_1 t1 t2 t1' h =
+let rec trapp_tss_1 #t1 t2 #t1' h =
   match h with
     | TssBase h1 -> TssBase (TrApp h1 (TrRefl t2))
     | TssSym h1 -> TssSym (trapp_tss_1 t2 h1)
@@ -965,7 +971,7 @@ let rec trapp_tss_1 t1 t2 t1' h =
 opaque val trapp_tss_2 : t1:typ -> #t2:typ -> #t2':typ ->
       h:(tred_star_sym t2 t2') ->
       Tot (tred_star_sym (TApp t1 t2) (TApp t1 t2')) (decreases h)
-let rec trapp_tss_2 t1 t2 t2' h =
+let rec trapp_tss_2 t1 #t2 #t2' h =
   match h with
     | TssBase h1 -> TssBase (TrApp (TrRefl t1) h1)
     | TssSym h1 -> TssSym (trapp_tss_2 t1 h1)
@@ -975,7 +981,7 @@ let rec trapp_tss_2 t1 t2 t2' h =
 opaque val trarr_tss_1 : #t1:typ -> t2:typ -> #t1':typ ->
       h:(tred_star_sym t1 t1') ->
       Tot (tred_star_sym (TArr t1 t2) (TArr t1' t2)) (decreases h)
-let rec trarr_tss_1 t1 t2 t1' h =
+let rec trarr_tss_1 #t1 t2 #t1' h =
   match h with
     | TssBase h1 -> TssBase (TrArr h1 (TrRefl t2))
     | TssSym h1 -> TssSym (trarr_tss_1 t2 h1)
@@ -984,7 +990,7 @@ let rec trarr_tss_1 t1 t2 t1' h =
 opaque val trarr_tss_2 : t1:typ -> #t2:typ -> #t2':typ ->
       h:(tred_star_sym t2 t2') ->
       Tot (tred_star_sym (TArr t1 t2) (TArr t1 t2')) (decreases h)
-let rec trarr_tss_2 t1 t2 t2' h =
+let rec trarr_tss_2 t1 #t2 #t2' h =
   match h with
     | TssBase h1 -> TssBase (TrArr (TrRefl t1) h1)
     | TssSym h1 -> TssSym (trarr_tss_2 t1 h1)
@@ -993,7 +999,7 @@ let rec trarr_tss_2 t1 t2 t2' h =
 (* LTR direction of Lemma 30.3.5 in TAPL; proof there is informal and unclear. *)
 opaque val tequiv_tss : #s:typ -> #t:typ -> h:(tequiv s t) ->
       Tot (tred_star_sym s t) (decreases h)
-let rec tequiv_tss s t h =
+let rec tequiv_tss #s #t h =
   match h with
   | EqRefl _ -> TssBase (TrRefl s)
   | EqSymm h1 -> TssSym (tequiv_tss h1)
@@ -1012,11 +1018,11 @@ let rec tequiv_tss s t h =
 opaque val tequiv_tred_tred : #s:typ -> #t:typ ->
       tequiv s t ->
       Tot (cexists (fun u -> cand (tred_star s u) (tred_star t u)))
-let tequiv_tred_tred s t h = tred_star_sym_confluent (tequiv_tss h)
+let tequiv_tred_tred #s #t h = tred_star_sym_confluent (tequiv_tss h)
 
 opaque val tred_tequiv : #s:typ -> #t:typ -> h:(tred s t) ->
                   Tot (tequiv s t) (decreases h)
-let rec tred_tequiv s t h =
+let rec tred_tequiv #s #t h =
   match h with
   | TrRefl _ -> EqRefl s
   | TrArr h1 h2 -> EqArr (tred_tequiv h1) (tred_tequiv h2)
@@ -1028,7 +1034,7 @@ let rec tred_tequiv s t h =
 
 opaque val tred_star_tequiv : #s:typ -> #t:typ -> h:(tred_star s t) ->
                        Tot (tequiv s t) (decreases h)
-let rec tred_star_tequiv s t h = match h with
+let rec tred_star_tequiv #s #t h = match h with
   | TsRefl _ -> EqRefl s
   | TsStep h1 h2 -> EqTran (tred_tequiv h1) (tred_star_tequiv h2)
 
@@ -1036,7 +1042,7 @@ let rec tred_star_tequiv s t h = match h with
    We don't use this anywhere *)
 opaque val tss_tequiv : #s:typ -> #t:typ ->
       h:(tred_star_sym s t) -> Tot (tequiv s t) (decreases h)
-let rec tss_tequiv s t h =
+let rec tss_tequiv #s #t h =
   match h with
     | TssBase h1 -> tred_tequiv h1
     | TssSym h1 -> EqSymm (tss_tequiv h1)
@@ -1048,7 +1054,7 @@ opaque val tred_tarr_preserved : #s1:typ -> #s2:typ -> #t:typ ->
       Tot (cexists (fun t1 -> (cexists (fun t2 ->
             (u:(cand (tred_star s1 t1) (tred_star s2 t2)){t = TArr t1 t2})))))
       (decreases h)
-let rec tred_tarr_preserved s1 s2 t h =
+let rec tred_tarr_preserved #s1 #s2 #t h =
   match h with
     | TsRefl _ -> ExIntro s1 (ExIntro s2 (Conj (TsRefl s1) (TsRefl s2)))
     | TsStep #s #u #t h1 hs1 ->
@@ -1059,6 +1065,7 @@ let rec tred_tarr_preserved s1 s2 t h =
             let ExIntro t1 (ExIntro t2 (Conj p1 p2)) =
                                            tred_tarr_preserved #u1 #u2 #t hs1 in
             ExIntro t1 (ExIntro t2 (Conj (TsStep h11 p1) (TsStep h12 p2)))
+
 //NS: Something seems super fragile here ...
 opaque val inversion_elam :
       #g:env -> s1:typ -> e:exp -> #s:typ -> t1:typ -> t2:typ ->
@@ -1066,7 +1073,7 @@ opaque val inversion_elam :
       hnew:kinding g t2 KTyp ->
       Tot (cand (cand (tequiv t1 s1) (typing (extend_evar g 0 s1) e t2))
                 (kinding g s1 KTyp))  (decreases ht)
-let rec inversion_elam g s1 e s t1 t2 ht heq hnew = match ht with
+let rec inversion_elam #g s1 e #s t1 t2 ht heq hnew = match ht with
   | TyEqu #g #e' #u #s ht1 heq1 k1 ->
     inversion_elam s1 e t1 t2 ht1 (EqTran heq1 heq) hnew
   | TyLam #g s1 #e #s2 hk ht1 ->
@@ -1115,6 +1122,7 @@ let rec inversion_elam g s1 e s t1 t2 ht heq hnew = match ht with
       TyEqu ht1 pst2 (kinding_weakening_ebnd hnew 0 s1) in
     Conj (Conj (EqTran (tred_star_tequiv ptu1)
                        (EqSymm (tred_star_tequiv psu1))) h) hk
+
 #reset-options
 
 (* Corollary of inversion_elam *)
@@ -1122,7 +1130,7 @@ opaque val inversion_elam_typing : #g:env -> s1:typ -> e:exp ->
       t1:typ -> t2:typ -> typing g (ELam s1 e) (TArr t1 t2) ->
       Tot (cand (cand (tequiv t1 s1) (typing (extend_evar g 0 s1) e t2))
                 (kinding g s1 KTyp))
-let inversion_elam_typing g s1 e t1 t2 h =
+let inversion_elam_typing #g s1 e t1 t2 h =
   inversion_elam s1 e t1 t2 h (EqRefl (TArr t1 t2))
     (Conj.h2 (kinding_inversion_arrow #g #t1 #t2 (typing_to_kinding h)))
 
@@ -1130,7 +1138,7 @@ let inversion_elam_typing g s1 e t1 t2 h =
 opaque val preservation : #e:exp -> #e':exp -> hs:step e e' ->
                    #g:env -> #t:typ -> ht:(typing g e t) ->
                    Tot (typing g e' t) (decreases ht)
-let rec preservation _ _ hs _ _ ht =
+let rec preservation #e #e' hs #g #t ht =
   match ht with
   | TyApp #g #e1 #e2 #t1 #t2 h1 h2 ->
     (match hs with
